Added second example.

Experiments.thy
@@ -9,9 +9,9 @@ begin
          prec - The floating point precision.
    expression - The floatarith expression used.
        domain - The domain we test on. 
-     tm_order - Order of the taylor models generated. *) 
-definition "n = 0"
-definition "prec = 32"
+     tm_order - Order of the taylor models generated. *)
+definition "n = 3"
+definition "prec = 64"
 definition "expression = (Add (Power (Cos (Var 0)) 2) (Power (Sin (Var 0)) 2))"
 definition "domain = [Ivl 0 10]"
 definition "tm_order = 7"
@@ -27,5 +27,53 @@ value "test_tm ()"
 
 ML \<open>Timing.timeit test_ia\<close>
 ML \<open>Timing.timeit test_tm\<close>
+
+(* The caprasse example from file thys/Affine_Arithmetic/Ex_Ineqs.thy in the AFP.  *)
+definition "caprasse = (\<lambda>x1 x2 x3 x4::real.
+  (- x1 * x3 * x3 * x3 + 4 * x2 * x3 * x3 * x4 +
+    4 * x1 * x3 * x4 * x4 + 2 * x2 * x4 * x4 * x4 + 4 * x1 * x3 + 4 * x3 * x3 + - 10 * x2 * x4 +
+    -10 * x4 * x4 + 2))"
+definition "caprasse_fa =
+  (floatarith.Add
+       (floatarith.Add
+         (floatarith.Add
+           (floatarith.Add
+             (floatarith.Add
+               (floatarith.Add
+                 (floatarith.Add
+                   (floatarith.Add
+                     (Mult (Mult (Mult (Minus (Var 0)) (Var (Suc (Suc 0))))
+                             (Var (Suc (Suc 0))))
+                       (Var (Suc (Suc 0))))
+                     (Mult (Mult (Mult (Mult (Num (Float 4 0)) (Var (Suc 0))) (Var (Suc (Suc 0))))
+                             (Var (Suc (Suc 0))))
+                       (Var 3)))
+                   (Mult (Mult (Mult (Mult (Num (Float 4 0)) (Var 0)) (Var (Suc (Suc 0))))
+                           (Var 3))
+                     (Var 3)))
+                 (Mult (Mult (Mult (Mult (Num (Float 2 0)) (Var (Suc 0))) (Var 3)) (Var 3)) (Var 3)))
+               (Mult (Mult (Num (Float 4 0)) (Var 0)) (Var (Suc (Suc 0)))))
+             (Mult (Mult (Num (Float 4 0)) (Var (Suc (Suc 0)))) (Var (Suc (Suc 0)))))
+           (Mult (Mult (Minus (Num (Float 10 0))) (Var (Suc 0))) (Var 3)))
+         (Mult (Mult (Minus (Num (Float 10 0))) (Var 3)) (Var 3)))
+       (Num (Float 2 0)))
+"
+
+lemma "interpret_floatarith caprasse_fa [x\<^sub>1, x\<^sub>2, x\<^sub>3, x\<^sub>4] = caprasse x\<^sub>1 x\<^sub>2 x\<^sub>3 x\<^sub>4"
+by (simp add: caprasse_fa_def caprasse_def power2_eq_square)
+
+definition "domain2 = (\<lambda>d. [d, d, d, d]) (Ivl (-10) 10)"
+  
+definition "test_ia2 (u::unit) = compute_bound_fa_via_ia prec n caprasse_fa domain2"
+definition "test_tm2 (u::unit) = compute_bound_fa_via_tm' prec tm_order n caprasse_fa domain2"
+
+ML \<open>val test_ia2 = @{code test_ia2}\<close>
+ML \<open>val test_tm2 = @{code test_tm2}\<close>
+
+value "test_ia2 ()"
+value "test_tm2 ()"
+
+ML \<open>Timing.timeit test_ia2\<close>
+ML \<open>Timing.timeit test_tm2\<close>
 
 end
